Progress on RightPass step

Refinement.thy
@@ -1,5 +1,5 @@
 theory Refinement
-  imports "Collections.Refine_Dflt_Only_ICF" LayerMaintenance
+  imports (*"Collections.Refine_Dflt_Only_ICF"*) "Refine_Monadic.Refine_Monadic" LayerMaintenance
 begin
 
 subsection \<open>PathFinding\<close>
@@ -77,8 +77,17 @@ subsection \<open>RightPass\<close>
 definition removeEdge :: "_ graph \<Rightarrow> edge \<Rightarrow> _ graph" where
   "removeEdge c e \<equiv> c(e := 0)"
 
-definition removeEdges :: "_graph \<Rightarrow> edge set \<Rightarrow> _ graph" where
+definition removeEdges :: "_ graph \<Rightarrow> edge set \<Rightarrow> _ graph" where
   "removeEdges c R \<equiv> \<lambda>e. if e \<in> R then 0 else c e"
+
+context Graph
+begin
+lemma removeEdges_subgraph: "isSubgraph (removeEdges c S) c"
+  unfolding removeEdges_def isSubgraph_def by presburger
+
+lemma removeEdges_E: "Graph.E (removeEdges c S) = E - S"
+  unfolding removeEdges_def Graph.E_def by auto
+end
 
 (* TODO refine removeEdges and use the refined version *)
 
@@ -137,9 +146,11 @@ definition rightPass_invar :: "_ graph \<Rightarrow> node \<Rightarrow> (_ graph
 
 definition rightPass_invar :: "_ graph \<Rightarrow> node \<Rightarrow> (_ graph \<times> node set) \<Rightarrow> bool"
   where "rightPass_invar c s \<equiv> \<lambda>(c', Q). isSubgraph c' c
+                                \<and> s \<notin> Q
                                 \<and> (\<forall>u v. Graph.connected c s u \<longrightarrow> Graph.connected c' s u \<and> c' (u, v) = c (u, v))
                                 \<and> (\<forall>u \<in> Graph.V c' - Q - {s}. Graph.incoming c' u \<noteq> {})"
 (* TODO check whether subgraph is necessary *)
+(* TODO check whether s \<notin> Q is necessary *)
 
 thm rightPassAbstract_def
 thm Graph.outgoing'_def
@@ -151,21 +162,50 @@ find_theorems "(?a \<noteq> 0 \<Longrightarrow> ?a = ?b) \<Longrightarrow> (?b \
 context Distance_Bounded_Graph
 begin
 
+lemma rightPassRefine_final:
+  assumes SUB: "isSubgraph c' c"
+    and S_CON: "\<And>u v. connected s u \<Longrightarrow> Graph.connected c' s u \<and> c' (u, v) = c (u, v)"
+    and NODE_HAS_IN: "\<forall>u \<in> Graph.V c' - {s}. Graph.incoming c' u \<noteq> {}"
+  shows "rightPassAbstract c s = c'"
+proof (intro subgraph.order_antisym, unfold isSubgraph_def, clarsimp_all)
+  fix u v
+  assume "rightPassAbstract c s (u, v) \<noteq> 0"
+  with S_CON show "rightPassAbstract c s (u, v) = c' (u, v)"
+    using rightPassAbstract_nz_iff S_Graph.rp_is_c_if_s_connected by metis
+next
+  interpret g': Distance_Bounded_Graph c' b
+    using SUB Subgraph.intro Subgraph.sg_Distance_Bounded Distance_Bounded_Graph_axioms by blast
+  fix u v
+  assume "c' (u, v) \<noteq> 0"
+  then have "u \<in> g'.V" unfolding Graph.V_def Graph.E_def by blast
+  obtain w where W_CON: "g'.connected w u" and W_NO_IN: "g'.incoming w = {}" using g'.obtain_front_terminal_connected by blast
+  from W_CON \<open>u \<in> g'.V\<close> have "w \<in> g'.V" by (meson g'.connected_inV_iff)
+  with W_NO_IN NODE_HAS_IN have "w = s" by blast
+  with W_CON have "rightPassAbstract c s (u, v) = c (u, v)"
+    using SUB Subgraph.intro Subgraph.sg_connected_remains_base_connected S_Graph.rp_is_c_if_s_connected by blast
+  also from SUB \<open>c' (u, v) \<noteq> 0\<close> have "... = c' (u, v)" unfolding isSubgraph_def by metis
+  finally show "c' (u, v) = rightPassAbstract c s (u, v)" by simp
+qed (* TODO cleanup *)
+
+find_theorems "?x \<notin> ?A \<Longrightarrow> ?x \<notin> ?B \<Longrightarrow> ?x \<notin> ?A \<union> ?B"
+
 theorem rightPassRefine_correct:
   (* TODO make sure the assumptions are correct *)
   (* TODO split into multiple lemma *)
-  assumes "s \<notin> Q" and NODE_HAS_IN: "\<forall>u \<in> V - Q - {s}. incoming u \<noteq> {}"
+  assumes S_NO_IN: "incoming s = {}"
+    and Q_START: "s \<notin> Q" "\<forall>u \<in> V - Q - {s}. incoming u \<noteq> {}"
   shows "rightPassRefine c Q \<le> RETURN (rightPassAbstract c s)"
   unfolding rightPassRefine_def
 proof (intro WHILE_rule[where I="rightPass_invar c s"] refine_vcg, clarsimp_all)
-  show "rightPass_invar c s (c, Q)" unfolding rightPass_invar_def using NODE_HAS_IN by blast
+  show "rightPass_invar c s (c, Q)" unfolding rightPass_invar_def using Q_START by blast
 next
   fix c' :: "'capacity graph"
   fix Q u
   assume "rightPass_invar c s (c', Q)" (*TODO needed? *)"u \<in> Q"
   then have SUB: "isSubgraph c' c"
+    and "s \<notin> Q"
     and S_CON: "\<And>u v. connected s u \<Longrightarrow> Graph.connected c' s u \<and> c' (u, v) = c (u, v)"
-    and NODE_HAS_IN': "\<forall>u \<in> Graph.V c' - Q - {s}. Graph.incoming c' u \<noteq> {}"
+    and NODE_HAS_IN: "\<forall>u \<in> Graph.V c' - Q - {s}. Graph.incoming c' u \<noteq> {}"
     unfolding rightPass_invar_def by simp_all
   then show "Graph.incoming c' u \<noteq> {} \<Longrightarrow> rightPass_invar c s (c', Q - {u})"
     unfolding rightPass_invar_def by blast
@@ -174,36 +214,37 @@ next
     (* TODO is distance bounded needed? *)
     (*interpret g': Distance_Bounded_Graph c' b using SUB Subgraph.intro Subgraph.sg_Distance_Bounded Distance_Bounded_Graph_axioms by blast*)
     interpret g': Graph c' .
+    interpret g'': Graph "removeEdges c' (g'.outgoing u)" .
+    (* abbreviation "c'' = removeEdges c' (g'.outgoing u)" *)
     assume "g'.incoming u = {}"
-    then show "rightPass_invar c s (removeEdges c' (g'.outgoing u), Q - {u} \<union> snd ` g'.outgoing u)" sorry
+    have "isSubgraph (removeEdges c' (g'.outgoing u)) c"
+      using g'.removeEdges_subgraph SUB subgraph.order_trans by blast
+    moreover have "s \<notin> Q - {u} \<union> snd ` g'.outgoing u"
+    proof -
+      from SUB S_NO_IN have "g'.incoming s = {}" unfolding Graph.incoming_def
+        using Subgraph.E_ss Subgraph.intro by fastforce
+      then have "s \<notin> snd ` g'.outgoing u" unfolding g'.incoming_def g'.outgoing_def by fastforce
+      with \<open>s \<notin> Q\<close> show ?thesis by blast
+    qed
+    moreover have "(\<forall>v w. connected s v \<longrightarrow> g''.connected s v \<and> (removeEdges c' (g'.outgoing u)) (v, w) = c (v, w))"
+    proof (clarify, intro conjI)
+      fix v w
+      assume "connected s v"
+      then have "g'.connected s v" "c' (v, w) = c (v, w)" using S_CON by simp_all
+      then obtain p where "g'.isPath s p v" unfolding g'.connected_def by blast
+      show "g''.connected s v" sorry
+      have "v \<noteq> u" sorry
+      then have "removeEdges c' (g'.outgoing u) (v, w) = c' (v, w)"
+        unfolding g'.outgoing_def removeEdges_def by simp
+      show "removeEdges c' (g'.outgoing u) (v, w) = c (v, w)" sorry
+    qed
+    moreover have "(\<forall>v \<in> g''.V - (Q - {u} \<union> snd ` g'.outgoing u) - {s}. g''.incoming v \<noteq> {})" sorry
+    ultimately show "rightPass_invar c s (removeEdges c' (g'.outgoing u), Q - {u} \<union> snd ` g'.outgoing u)" unfolding rightPass_invar_def by simp
   qed
 next
   fix c' :: "'capacity  graph"
   assume "rightPass_invar c s (c', {})"
-  then have SUB: "isSubgraph c' c"
-    and S_CON: "\<And>u v. connected s u \<Longrightarrow> Graph.connected c' s u \<and> c' (u, v) = c (u, v)"
-    and NODE_HAS_IN': "\<forall>u \<in> Graph.V c' - {s}. Graph.incoming c' u \<noteq> {}"
-    unfolding rightPass_invar_def by simp_all
-  show "rightPassAbstract c s = c'"
-  proof (intro subgraph.order_antisym, unfold isSubgraph_def, clarsimp_all)
-    fix u v
-    assume "rightPassAbstract c s (u, v) \<noteq> 0"
-    with S_CON show "rightPassAbstract c s (u, v) = c' (u, v)"
-      using rightPassAbstract_nz_iff S_Graph.rp_is_c_if_s_connected by metis
-  next
-    interpret g': Distance_Bounded_Graph c' b
-      using SUB Subgraph.intro Subgraph.sg_Distance_Bounded Distance_Bounded_Graph_axioms by blast
-    fix u v
-    assume "c' (u, v) \<noteq> 0"
-    then have "u \<in> g'.V" unfolding Graph.V_def Graph.E_def by blast
-    obtain w where W_CON: "g'.connected w u" and W_NO_IN: "g'.incoming w = {}" using g'.obtain_front_terminal_connected by blast
-    from W_CON \<open>u \<in> g'.V\<close> have "w \<in> g'.V" by (meson g'.connected_inV_iff)
-    with W_NO_IN NODE_HAS_IN' have "w = s" by blast
-    with W_CON have "rightPassAbstract c s (u, v) = c (u, v)"
-      using SUB Subgraph.intro Subgraph.sg_connected_remains_base_connected S_Graph.rp_is_c_if_s_connected by blast
-    also from SUB \<open>c' (u, v) \<noteq> 0\<close> have "... = c' (u, v)" unfolding isSubgraph_def by metis
-    finally show "c' (u, v) = rightPassAbstract c s (u, v)" by simp
-  qed
+  then show "rightPassAbstract c s = c'" unfolding rightPass_invar_def using rightPassRefine_final by simp
 qed
 end
 
